Prove cComp generates code_locs
Required tweaking the definition of code_locs (and renumber_code_locs)
so that it does things in exactly the same order as cComp. Unfortunately
also required changing cComp to be self-consistent in its ordering (the
special case of Letrec differed from the general case).

new-backend/clos_numberScript.sml
@@ -67,11 +67,11 @@ val code_locs_def = tDefine "code_locs" `
          c1++c2) /\
   (code_locs [Fn loc vs x1] =
      let c1 = code_locs [x1] in
-       loc::c1) /\
+       c1 ++ [loc]) /\
   (code_locs [Letrec loc vs fns x1] =
      let c1 = code_locs fns in
      let c2 = code_locs [x1] in
-     GENLIST ($+ loc) (LENGTH fns) ++ c1 ++ c2) /\
+     c1 ++ GENLIST ($+ loc) (LENGTH fns) ++ c2) /\
   (code_locs [Handle x1 x2] =
      let c1 = code_locs [x1] in
      let c2 = code_locs [x2] in
@@ -115,12 +115,12 @@ val renumber_code_locs_def = tDefine "renumber_code_locs" `
      let (n,x2) = renumber_code_locs n x2 in
        (n,App loc_opt x1 x2)) /\
   (renumber_code_locs n (Fn loc vs x1) =
-     let (m,x1) = renumber_code_locs (n+1) x1 in
-       (m,Fn n vs x1)) /\
+     let (n,x1) = renumber_code_locs n x1 in
+       (n+1,Fn n vs x1)) /\
   (renumber_code_locs n (Letrec loc vs fns x1) =
-     let (m,fns) = renumber_code_locs_list (n+LENGTH fns) fns in
-     let (m,x1) = renumber_code_locs m x1 in
-     (m,Letrec n vs fns x1)) /\
+     let (m,fns) = renumber_code_locs_list n fns in
+     let (n,x1) = renumber_code_locs (m+LENGTH fns) x1 in
+     (n,Letrec m vs fns x1)) /\
   (renumber_code_locs n (Handle x1 x2) =
      let (n,x1) = renumber_code_locs n x1 in
      let (n,x2) = renumber_code_locs n x2 in
@@ -157,14 +157,8 @@ val renumber_code_locs_inc = store_thm("renumber_code_locs_inc",
   simp[renumber_code_locs_def] >> rw[] >>
   tac >> fs[] >>
   tac >> fs[] >>
-  tac >> fs[] >> simp[]
-  >- (
-    Cases_on`renumber_code_locs (n+1) e` >> fs[] >>
-    simp[] )
-  >- (
-    Cases_on`renumber_code_locs_list (n+LENGTH es) es` >> fs[] >>
-    tac >> fs[] >>
-    simp[] ))
+  tac >> fs[] >> simp[] >>
+  Cases_on`renumber_code_locs (q+LENGTH r) e`>>fs[]>>simp[])
 
 val renumber_code_locs_imp_inc = prove(
   ``(renumber_code_locs_list n es = (m,vs) ⇒ n ≤ m) ∧
@@ -226,7 +220,7 @@ val renumber_code_locs_distinct_lemma = prove(
     imp_res_tac renumber_code_locs_imp_inc >>
     rw[] >> fs[EVERY_MEM] >> res_tac >> fsrw_tac[ARITH_ss][] >>
     NO_TAC) >>
-  Cases_on`renumber_code_locs_list (n+LENGTH es) es`>>fs[] >>
+  Cases_on`renumber_code_locs (q+LENGTH r) e`>>fs[] >>
   rpt(CHANGED_TAC tac >> fs[])>>
   simp[SORTED_GENLIST_PLUS] >>
   simp[MEM_GENLIST] >>
@@ -474,14 +468,14 @@ val renumber_code_locs_correct = store_thm("renumber_code_locs_correct",
       imp_res_tac LIST_REL_LENGTH >>
       DECIDE_TAC ) >>
     fs[LIST_REL_EL_EQN] >>
-    qexists_tac`n+1`>>simp[] >>
+    qexists_tac`n`>>simp[] >>
     imp_res_tac lookup_vars_SOME >>
     imp_res_tac lookup_vars_MEM >>
     simp[] )
   THEN1 (* Letrec *)
    (fs[renumber_code_locs_def,cEval_def,LET_THM,UNCURRY] >>
     `t1.restrict_envs = s.restrict_envs` by fs[state_rel_def] >>
-    Cases_on`renumber_code_locs_list (n+LENGTH fns) fns`>>fs[]>>
+    Cases_on`renumber_code_locs_list n fns`>>fs[]>>
     fs[build_recc_def,clos_env_def] >> reverse(rw[]) >> fs[contains_App_SOME_def] >> rw[] >- (
       first_x_assum MATCH_MP_TAC >> rw[] >>
       MATCH_MP_TAC EVERY2_APPEND_suff >> rw[] >>
@@ -507,7 +501,7 @@ val renumber_code_locs_correct = store_thm("renumber_code_locs_correct",
       rw[val_rel_simp,LIST_REL_EL_EQN] >>
       imp_res_tac lookup_vars_SOME >>
       imp_res_tac lookup_vars_MEM >>
-      qexists_tac`n + LENGTH fns`>>simp[] >>
+      qexists_tac`n`>>simp[] >>
       fs[LIST_REL_EL_EQN]) >>
     imp_res_tac lookup_vars_NONE >>
     imp_res_tac lookup_vars_SOME >>
